progress in reduction proof + cleanup + proof and draft theories compile now

txn-data-consistency/EP+.thy
@@ -226,9 +226,16 @@ definition ects :: "tstmp \<Rightarrow> cl_id \<Rightarrow> tstmp \<times> cl_id
 lemma ects_inj: "ects cts cl = ects cts' cl' \<Longrightarrow> cts = cts' \<and> cl = cl'"
   by (simp add: ects_def)
 
+lemma min_ects: "(0, 0) < ects x y" by (auto simp add: less_prod_def ects_def)
+
 fun ev_ects :: "'v ev \<Rightarrow> (tstmp \<times> cl_id) option" where
   "ev_ects (WCommit cl kv_map cts sn u'') = Some (ects cts cl)" |
   "ev_ects _ = None"
+
+lemma ev_ects_Some:
+  "ev_ects e = Some (cts, Suc_cl)
+  \<Longrightarrow> \<exists>cl kv_map sn u''. e = WCommit cl kv_map cts sn u'' \<and> Suc_cl = Suc cl"
+  by (cases e, simp_all add: ects_def)
 
 definition unique_ts :: "(txid \<rightharpoonup> tstmp) \<Rightarrow> txid \<Rightarrow> tstmp \<times> cl_id" where
   "unique_ts wtxn_ctss \<equiv> (\<lambda>t. (the (wtxn_ctss t), if t = T0 then 0 else Suc (get_cl_w t)))"
@@ -505,82 +512,5 @@ lemmas tps_trans_all_defs = tps_trans_defs ext_corder_def
 lemmas tps_defs = tps_def state_init_def
 
 lemma tps_trans [simp]: "trans tps = state_trans" by (simp add: tps_def)
-
-
-subsection \<open>Invariants - needed for reduction\<close>
-
-text \<open>Invariants\<close>
-
-definition Wtxn_Cts_Tn_None where
-  "Wtxn_Cts_Tn_None s \<longleftrightarrow> (\<forall>cts kv_map keys n cl. 
-    (cl_state (cls s cl) \<in> {Idle, WtxnPrep kv_map} \<and> n \<ge> cl_sn (cls s cl)) \<or>
-    (cl_state (cls s cl) \<in> {RtxnInProg keys kv_map, WtxnCommit cts kv_map} \<and> n > cl_sn (cls s cl))
-     \<longrightarrow> wtxn_cts s (Tn (Tn_cl n cl)) = None)"
-
-lemmas Wtxn_Cts_Tn_NoneI = Wtxn_Cts_Tn_None_def[THEN iffD2, rule_format]
-lemmas Wtxn_Cts_Tn_NoneE[elim] = Wtxn_Cts_Tn_None_def[THEN iffD1, elim_format, rule_format]
-
-lemma reach_wtxn_cts_tn_none [simp, intro]: "reach tps s \<Longrightarrow> Wtxn_Cts_Tn_None s"
-proof(induction s rule: reach.induct)
-  case (reach_init s)
-  then show ?case
-    by (auto simp add: Wtxn_Cts_Tn_None_def tps_defs)
-next
-  case (reach_trans s e s')
-  then show ?case
-    by (induction e) (auto simp add: Wtxn_Cts_Tn_None_def tps_trans_defs)
-qed
-
-definition Wtxn_Cts_None where
-  "Wtxn_Cts_None s \<longleftrightarrow> (\<forall>cts kv_map keys t. t \<noteq> T0 \<and> (
-    (cl_state (cls s (get_cl_w t)) \<in> {Idle, WtxnPrep kv_map} \<and>
-        get_sn_w t \<ge> cl_sn (cls s (get_cl_w t))) \<or>
-    (cl_state (cls s (get_cl_w t)) \<in> {RtxnInProg keys kv_map, WtxnCommit cts kv_map} \<and>
-        get_sn_w t > cl_sn (cls s (get_cl_w t))))
-     \<longrightarrow> wtxn_cts s t = None)"
-
-lemmas Wtxn_Cts_NoneI = Wtxn_Cts_None_def[THEN iffD2, rule_format]
-lemmas Wtxn_Cts_NoneE[elim] = Wtxn_Cts_None_def[THEN iffD1, elim_format, rule_format]
-
-lemma reach_wtxn_cts_none [simp, intro]: "reach tps s \<Longrightarrow> Wtxn_Cts_None s"
-  apply (simp add: Wtxn_Cts_None_def)
-  apply rule+ subgoal for cts kv_map keys t apply (cases t)
-    apply metis using Wtxn_Cts_Tn_None_def[of s]
-    by (smt get_cl_w.simps(2) get_sn_w.simps(2) insert_iff reach_wtxn_cts_tn_none txid0.exhaust).
-
-definition CO_Tid where
-  "CO_Tid s cl \<longleftrightarrow> (case cl_state (cls s cl) of
-    WtxnCommit cts kv_map \<Rightarrow> (\<forall>k n. Tn (Tn_cl n cl) \<in> set (cts_order s k) \<longrightarrow> n \<le> cl_sn (cls s cl))
-  | _ \<Rightarrow> (\<forall>k n. Tn (Tn_cl n cl) \<in> set (cts_order s k) \<longrightarrow> n < cl_sn (cls s cl)))"
-
-lemmas CO_TidI = CO_Tid_def[THEN iffD2, rule_format]
-lemmas CO_TidE[elim] = CO_Tid_def[THEN iffD1, elim_format, rule_format]
-
-lemma reach_co_tid[simp]: "reach tps s \<Longrightarrow> CO_Tid s cl"
-proof(induction s rule: reach.induct)
-  case (reach_init s)
-  then show ?case
-    by (auto simp add: CO_Tid_def tps_defs)
-next
-  case (reach_trans s e s')
-  then show ?case
-  proof (induction e)
-    case (RDone x1 x2 x3 x4)
-    then show ?case apply (simp add: CO_Tid_def tps_trans_defs split: txn_state.split_asm)
-      using less_SucI less_Suc_eq_le by blast+
-  next
-    case (WCommit x1 x2 x3 x4 x5)
-    then show ?case apply (simp add: CO_Tid_def tps_trans_all_defs set_insort_key split: txn_state.split_asm)
-      apply (metis txn_state.distinct(3))
-      apply (metis txn_state.distinct(7))
-      apply (meson less_or_eq_imp_le)
-      by blast
-  next
-    case (WDone x1 x2)
-    then show ?case apply (simp add: CO_Tid_def tps_trans_defs split: txn_state.split_asm)
-      apply (meson less_SucI)+
-      by (meson linorder_le_less_linear not_less_eq_eq)
-  qed (auto simp add: CO_Tid_def tps_trans_defs split: txn_state.split_asm)
-qed
 
 end
