txn-data-consistency/EP+_Trace.thy
@@ -1,0 +1,193 @@
+section \<open>lemmas connecting the trace to tps states\<close>
+
+theory "EP+_Trace"
+  imports "EP+" Reductions
+begin
+
+subsubsection \<open>Invariants\<close>
+
+definition Wtxn_Cts_Tn_None where
+  "Wtxn_Cts_Tn_None s \<longleftrightarrow> (\<forall>cts kv_map keys n cl. 
+    (cl_state (cls s cl) \<in> {Idle, WtxnPrep kv_map} \<and> n \<ge> cl_sn (cls s cl)) \<or>
+    (cl_state (cls s cl) \<in> {RtxnInProg keys kv_map, WtxnCommit cts kv_map} \<and> n > cl_sn (cls s cl))
+     \<longrightarrow> wtxn_cts s (Tn (Tn_cl n cl)) = None)"
+
+lemmas Wtxn_Cts_Tn_NoneI = Wtxn_Cts_Tn_None_def[THEN iffD2, rule_format]
+lemmas Wtxn_Cts_Tn_NoneE[elim] = Wtxn_Cts_Tn_None_def[THEN iffD1, elim_format, rule_format]
+
+lemma reach_wtxn_cts_tn_none [simp, intro]: "reach tps s \<Longrightarrow> Wtxn_Cts_Tn_None s"
+proof(induction s rule: reach.induct)
+  case (reach_init s)
+  then show ?case
+    by (auto simp add: Wtxn_Cts_Tn_None_def tps_defs)
+next
+  case (reach_trans s e s')
+  then show ?case
+    by (induction e) (auto simp add: Wtxn_Cts_Tn_None_def tps_trans_defs)
+qed
+
+definition Wtxn_Cts_None where
+  "Wtxn_Cts_None s \<longleftrightarrow> (\<forall>cts kv_map keys t. t \<noteq> T0 \<and> (
+    (cl_state (cls s (get_cl_w t)) \<in> {Idle, WtxnPrep kv_map} \<and>
+        get_sn_w t \<ge> cl_sn (cls s (get_cl_w t))) \<or>
+    (cl_state (cls s (get_cl_w t)) \<in> {RtxnInProg keys kv_map, WtxnCommit cts kv_map} \<and>
+        get_sn_w t > cl_sn (cls s (get_cl_w t))))
+     \<longrightarrow> wtxn_cts s t = None)"
+
+lemmas Wtxn_Cts_NoneI = Wtxn_Cts_None_def[THEN iffD2, rule_format]
+lemmas Wtxn_Cts_NoneE[elim] = Wtxn_Cts_None_def[THEN iffD1, elim_format, rule_format]
+
+lemma reach_wtxn_cts_none [simp, intro]: "reach tps s \<Longrightarrow> Wtxn_Cts_None s"
+  apply (simp add: Wtxn_Cts_None_def)
+  apply rule+ subgoal for cts kv_map keys t apply (cases t)
+    apply metis using Wtxn_Cts_Tn_None_def[of s]
+    by (smt get_cl_w.simps(2) get_sn_w.simps(2) insert_iff reach_wtxn_cts_tn_none txid0.exhaust).
+
+definition Wtxn_Cts_T0 where
+  "Wtxn_Cts_T0 s k \<longleftrightarrow> wtxn_cts s T0 = Some 0"
+
+lemmas Wtxn_Cts_T0I = Wtxn_Cts_T0_def[THEN iffD2, rule_format]
+lemmas Wtxn_Cts_T0E[elim] = Wtxn_Cts_T0_def[THEN iffD1, elim_format, rule_format]
+
+lemma reach_wtxn_cts_t0 [simp, dest]: "reach tps s \<Longrightarrow> Wtxn_Cts_T0 s k"
+proof(induction s rule: reach.induct)
+  case (reach_init s)
+  then show ?case
+    by (auto simp add: Wtxn_Cts_T0_def tps_defs)
+next
+  case (reach_trans s e s')
+  then show ?case
+    by (induction e) (auto simp add: Wtxn_Cts_T0_def tps_trans_defs)
+qed
+
+definition CO_Tid where
+  "CO_Tid s cl \<longleftrightarrow> (case cl_state (cls s cl) of
+    WtxnCommit cts kv_map \<Rightarrow> (\<forall>k n. Tn (Tn_cl n cl) \<in> set (cts_order s k) \<longrightarrow> n \<le> cl_sn (cls s cl))
+  | _ \<Rightarrow> (\<forall>k n. Tn (Tn_cl n cl) \<in> set (cts_order s k) \<longrightarrow> n < cl_sn (cls s cl)))"
+
+lemmas CO_TidI = CO_Tid_def[THEN iffD2, rule_format]
+lemmas CO_TidE[elim] = CO_Tid_def[THEN iffD1, elim_format, rule_format]
+
+lemma reach_co_tid[simp]: "reach tps s \<Longrightarrow> CO_Tid s cl"
+proof(induction s rule: reach.induct)
+  case (reach_init s)
+  then show ?case
+    by (auto simp add: CO_Tid_def tps_defs)
+next
+  case (reach_trans s e s')
+  then show ?case
+  proof (induction e)
+    case (RDone x1 x2 x3 x4)
+    then show ?case apply (simp add: CO_Tid_def tps_trans_defs split: txn_state.split_asm)
+      using less_SucI less_Suc_eq_le by blast+
+  next
+    case (WCommit x1 x2 x3 x4 x5)
+    then show ?case apply (simp add: CO_Tid_def tps_trans_all_defs set_insort_key split: txn_state.split_asm)
+      apply (metis txn_state.distinct(3))
+      apply (metis txn_state.distinct(7))
+      apply (meson less_or_eq_imp_le)
+      by blast
+  next
+    case (WDone x1 x2)
+    then show ?case apply (simp add: CO_Tid_def tps_trans_defs split: txn_state.split_asm)
+      apply (meson less_SucI)+
+      by (meson linorder_le_less_linear not_less_eq_eq)
+  qed (auto simp add: CO_Tid_def tps_trans_defs split: txn_state.split_asm)
+qed
+
+definition Dom_Kv_map_non_Emp where
+  "Dom_Kv_map_non_Emp s cl \<longleftrightarrow>
+    (\<forall>kv_map cts. cl_state (cls s cl) \<in> {WtxnPrep kv_map, WtxnCommit cts kv_map} \<longrightarrow>
+      (\<exists>k v. kv_map k = Some v))"
+                                                           
+lemmas Dom_Kv_map_non_EmpI = Dom_Kv_map_non_Emp_def[THEN iffD2, rule_format]
+lemmas Dom_Kv_map_non_EmpE[elim] = Dom_Kv_map_non_Emp_def[THEN iffD1, elim_format, rule_format]
+         
+lemma reach_dom_kv_map_non_emp [simp]: "reach tps s \<Longrightarrow> Dom_Kv_map_non_Emp s cl"
+proof(induction s rule: reach.induct)
+  case (reach_init s)
+  then show ?case
+  by (auto simp add: Dom_Kv_map_non_Emp_def tps_defs)
+next
+  case (reach_trans s e s')
+  then show ?case
+    by (induction e) (auto simp add: Dom_Kv_map_non_Emp_def tps_trans_defs)
+qed
+
+subsection \<open>Lemmas\<close>
+
+lemma trace_cts_order_tps:
+  assumes
+    \<open>tps: s \<midarrow>\<langle>\<tau>\<rangle>\<rightarrow> s'\<close>
+    \<open>init tps s\<close>
+  shows "Tn (Tn_cl sn cl) \<in> set (cts_order s' k) \<longleftrightarrow>
+    (\<exists>kv_map cts u''. k \<in> dom kv_map \<and> WCommit cl kv_map cts sn u'' \<in> set \<tau>)"
+  using assms(1)
+proof (induction \<tau> s' rule: trace.induct)
+  case trace_nil
+  then show ?case using assms(2) by (simp add: tps_defs)
+next
+  case (trace_snoc \<tau> s' e s'')
+  then show ?case
+  proof (induction e)
+    case (WCommit x1 x2 x3 x4 x5)
+    then show ?case apply (simp add: tps_trans_all_defs set_insort_key)
+      by (metis domIff option.discI)
+  qed (auto simp add: tps_trans_defs)
+qed
+
+lemma wtxn_cts_immutable:
+  assumes
+    \<open>wtxn_cts s t = Some c\<close>
+    \<open>tps: s \<midarrow>e\<rightarrow> s'\<close>
+    \<open>reach tps s\<close>
+  shows
+    \<open>wtxn_cts s' t = Some c\<close>
+  using assms
+proof (induction e)
+  case (WCommit x1 x2 x3 x4 x5)
+  then show ?case apply (simp add: write_commit_def write_commit_U_def write_commit_G_def)
+    apply (cases "t = get_wtxn s x1", auto) using Wtxn_Cts_Tn_None_def
+    by (metis (lifting) reach_wtxn_cts_tn_none domI domIff insertCI less_imp_neq linorder_not_le)
+qed (auto simp add: tps_trans_defs)
+
+lemma WC_in_\<tau>_wtxn_cts:
+  assumes
+    \<open>tps: s \<midarrow>\<langle>\<tau>\<rangle>\<rightarrow> s'\<close>
+    \<open>init tps s\<close>
+    \<open>WCommit cl kv_map cts sn u'' \<in> set \<tau>\<close>
+  shows "wtxn_cts s' (Tn (Tn_cl sn cl)) = Some cts"
+  using assms
+proof (induction \<tau> s' arbitrary: cl kv_map cts sn u'' rule: trace.induct)
+  case (trace_snoc \<tau> s' e s'')
+  then show ?case
+  proof (induction e)
+    case (WCommit x1 x2 x3 x4 x5)
+    then show ?case apply (auto simp add: set_insort_key)
+      subgoal by (simp add: tps_trans_all_defs) 
+      subgoal using wtxn_cts_immutable[of s' "Tn (Tn_cl sn cl)" cts "WCommit x1 x2 x3 x4 x5" s'']
+        apply (simp add: trace_is_trace_of_exec_frag reach_last_exec valid_exec_def)
+        apply (cases "get_txn s' x1 = Tn_cl sn cl")
+        by (auto simp add: tps_trans_all_defs)
+      done
+  qed (auto simp add: tps_trans_defs)
+qed simp
+
+lemma WC_in_\<tau>_kv_map_non_emp:
+  assumes
+    \<open>tps: s \<midarrow>\<langle>\<tau>\<rangle>\<rightarrow> s'\<close>
+    \<open>init tps s\<close>
+    \<open>WCommit cl kv_map cts sn u'' \<in> set \<tau>\<close>
+  shows "\<exists>k v. kv_map k = Some v"
+  using assms
+proof (induction \<tau> s' arbitrary: cl kv_map cts sn u'' rule: trace.induct)
+  case (trace_snoc \<tau> s' e s'')
+  then show ?case
+  proof (induction e)
+    case (WCommit x1 x2 x3 x4 x5)
+    then show ?case using Dom_Kv_map_non_Emp_def[of s' x1]
+    by (auto simp add: reach_traceI tps_trans_defs)
+  qed (auto simp add: tps_trans_defs)
+qed simp
+
+end
